Flatten the structure of Identifier.v
This is in preparation for autogenerating most of Identifier.v

To allow most of the code to continue compiling without much
modification, all of the qualified names we used to have in Identifier.v
now exist as only-parsing notations in API.v.

src/Rewriter/Passes/ToFancyWithCasts.v
@@ -1,6 +1,7 @@
 Require Import Coq.ZArith.ZArith.
 Require Import Crypto.Util.ZRange.
 Require Import Crypto.Language.Language.
+Require Import Crypto.Language.API.
 Require Import Crypto.Language.Wf.
 Require Import Crypto.Language.WfExtra.
 Require Import Crypto.Rewriter.AllTacticsExtra.
@@ -8,8 +9,8 @@ Require Import Crypto.Rewriter.RulesProofs.
 
 Module Compilers.
   Import Language.Compilers.
+  Import Language.API.Compilers.
   Import Language.Wf.Compilers.
-  Import Identifier.Compilers.
   Import Language.WfExtra.Compilers.
   Import Rewriter.AllTactics.Compilers.RewriteRules.GoalType.
   Import Rewriter.AllTacticsExtra.Compilers.RewriteRules.Tactic.
@@ -25,7 +26,7 @@ Module Compilers.
       Definition VerifiedRewriterToFancyWithCasts : VerifiedRewriter.
       Proof using All. make_rewriter false (@fancy_with_casts_rewrite_rules_proofs invert_low invert_high value_range flag_range Hlow Hhigh). Defined.
 
-      Definition RewriteToFancyWithCasts {t} : Expr (ident:=ident) t -> Expr (ident:=ident) t.
+      Definition RewriteToFancyWithCasts {t} : API.Expr t -> API.Expr t.
       Proof using invert_low invert_high value_range flag_range.
         let v := (eval hnf in (@Rewrite VerifiedRewriterToFancyWithCasts t)) in exact v.
       Defined.
@@ -34,11 +35,11 @@ Module Compilers.
       Proof using All. now apply VerifiedRewriterToFancyWithCasts. Qed.
 
       Lemma Interp_gen_RewriteToFancyWithCasts {cast_outside_of_range t} e (Hwf : Wf e)
-        : expr.Interp (@ident.gen_interp cast_outside_of_range) (@RewriteToFancyWithCasts t e)
-          == expr.Interp (@ident.gen_interp cast_outside_of_range) e.
+        : API.gen_Interp cast_outside_of_range (@RewriteToFancyWithCasts t e)
+          == API.gen_Interp cast_outside_of_range e.
       Proof using All. now apply VerifiedRewriterToFancyWithCasts. Qed.
 
-      Lemma Interp_RewriteToFancyWithCasts {t} e (Hwf : Wf e) : expr.Interp (@ident.interp) (@RewriteToFancyWithCasts t e) == expr.Interp (@ident.interp) e.
+      Lemma Interp_RewriteToFancyWithCasts {t} e (Hwf : Wf e) : API.Interp (@RewriteToFancyWithCasts t e) == API.Interp e.
       Proof using All. apply Interp_gen_RewriteToFancyWithCasts; assumption. Qed.
     End __.
   End RewriteRules.
