src/Rewriter/AllTacticsExtra.v
@@ -1,18 +1,18 @@
 Require Import Crypto.Rewriter.AllTactics.
-Require Import Crypto.Language.Identifier.
+Require Import Crypto.Language.API.
 Require Import Crypto.Language.IdentifiersGENERATEDProofs.
 
 Module Compilers.
   Import IdentifiersGENERATEDProofs.Compilers.pattern.ident.
   Import Rewriter.AllTactics.Compilers.
-  Import Identifier.Compilers.
+  Import API.Compilers.
 
   Module RewriteRules.
     Module Export Tactic.
       Export Rewriter.AllTactics.Compilers.RewriteRules.Tactic.Settings.
 
       Ltac make_rewriter include_interp specs_proofs :=
-        Rewriter.AllTactics.Compilers.RewriteRules.Tactic.make_rewriter ltac:(Identifier.Compilers.base.reify_base) ltac:(Identifier.Compilers.ident.reify) Identifier.Compilers.Classes.exprInfo Identifier.Compilers.Classes.exprExtraInfo IdentifiersGENERATEDProofs.Compilers.pattern.ident.package_proofs Identifier.Compilers.ident.is_var_like include_interp specs_proofs.
+        Rewriter.AllTactics.Compilers.RewriteRules.Tactic.make_rewriter ltac:(API.Compilers.base.reify_base) ltac:(API.Compilers.ident.reify) API.Compilers.Classes.exprInfo API.Compilers.Classes.exprExtraInfo IdentifiersGENERATEDProofs.Compilers.pattern.ident.package_proofs API.Compilers.ident.is_var_like include_interp specs_proofs.
 
       Tactic Notation "make_rewriter" constr(include_interp) constr(specs_proofs) :=
         make_rewriter include_interp specs_proofs.
