src/Stringification/C.v
@@ -15,6 +15,7 @@ Require Import Crypto.Util.ZRange.Show.
 Require Import Crypto.Util.Option.
 Require Import Crypto.Util.OptionList.
 Require Import Crypto.Language.Language.
+Require Import Crypto.Language.API.
 Require Import Crypto.Stringification.Language.
 Require Import Crypto.Stringification.IR.
 Require Import Crypto.AbstractInterpretation.AbstractInterpretation.
@@ -27,10 +28,11 @@ Module Compilers.
   Local Set Boolean Equality Schemes.
   Local Set Decidable Equality Schemes.
   Export Language.Compilers.
+  Export Language.API.Compilers.
   Export AbstractInterpretation.Compilers.
   Export Stringification.Language.Compilers.
   Import invert_expr.
-  Import API.
+  Import Compilers.API.
 
   Module ToString.
     Import Stringification.Language.Compilers.ToString.
